1

Sequent.thy
@@ -37,7 +37,7 @@ datatype 'u form =
   | FF
 
 
-primrec eval :: \<open>'u var_denot \<Rightarrow> 'u fun_denot \<Rightarrow> 'u form \<Rightarrow> bool\<close> where
+primrec eval :: \<open>'u var_denot \<Rightarrow> 'u fun_denot \<Rightarrow> 'u BA form \<Rightarrow> bool\<close> where
   "eval e f (EqAtom x y) = (evalt e f x = evalt e f y)" 
 | "eval e f (NeqAtom x y) = (evalt e f x \<noteq> evalt e f y)" 
 | "eval e f (Member x r) = ([evalt e f x] \<in> lang r)"
@@ -47,19 +47,19 @@ primrec eval :: \<open>'u var_denot \<Rightarrow> 'u fun_denot \<Rightarrow> 'u 
 | "eval e f (Neg m) = (\<not> eval e f m)"
 | "eval e f FF = False"
 
-definition model :: \<open>'u var_denot \<Rightarrow> 'u fun_denot \<Rightarrow>  'u form list \<Rightarrow> 'u form \<Rightarrow> bool\<close> ("_,_,_ \<Turnstile> _" [50,50] 50) where
+definition model :: \<open>'u var_denot \<Rightarrow> 'u fun_denot \<Rightarrow>  'u BA form list \<Rightarrow> 'u BA form \<Rightarrow> bool\<close> ("_,_,_ \<Turnstile> _" [50,50] 50) where
   \<open>(e,f,ps \<Turnstile> p) = (list_all (eval e f) ps \<longrightarrow> eval e f p)\<close>
 
-fun pre_image_conc ::"'u rexp \<Rightarrow> ('u rexp * 'u rexp) set" where 
+fun pre_image_conc ::"'u BA rexp \<Rightarrow> ('u BA rexp * 'u BA rexp) set" where 
   "pre_image_conc r = {(a,b)| a b. lang r = (lang (Times a b))}"
 
-fun empty_intersection_set :: "'u rexp list \<Rightarrow> bool" where
+fun empty_intersection_set :: "'u BA rexp list \<Rightarrow> bool" where
   "empty_intersection_set fs = (\<Inter>(lang ` set fs) = {} \<and> length fs > 1 )"
 
-fun subset_intersect_set :: "'u rexp \<Rightarrow> 'u rexp set \<Rightarrow> bool" where 
+fun subset_intersect_set :: "'u BA rexp \<Rightarrow> 'u BA rexp set \<Rightarrow> bool" where 
   "subset_intersect_set r fs = (\<Inter>(lang ` fs) \<subseteq> lang r)"
 
-fun eq_len_intersect :: "'u rexp \<Rightarrow> 'u rexp list \<Rightarrow> bool" where 
+fun eq_len_intersect :: "'u BA rexp \<Rightarrow> 'u BA rexp list \<Rightarrow> bool" where 
   "eq_len_intersect r fs = (\<Inter>(lang ` set fs) = lang r \<and> length fs > 1)"
 
 fun member_var_rexp :: "string list\<Rightarrow> 'u rexp list \<Rightarrow> 'u form set" where 
@@ -67,20 +67,20 @@ fun member_var_rexp :: "string list\<Rightarrow> 'u rexp list \<Rightarrow> 'u f
 "member_var_rexp (v # va) [] = {}"|
 "member_var_rexp (x#xs) (y#ys) = (if (length xs = length ys) then insert (Member (Var x) (y)) (member_var_rexp xs (ys)) else {})"
 
-fun con_fwd_prop ::"string \<Rightarrow> 'u rexp \<Rightarrow> 'u rexp list \<Rightarrow> bool" where
+fun con_fwd_prop ::"string \<Rightarrow> 'u BA rexp \<Rightarrow> 'u BA rexp list \<Rightarrow> bool" where
 "con_fwd_prop f r es = (if f = ''concat'' then lang (r) = List.foldl (*) (lang (hd es)) (map lang (tl es)) else False)"
 
-fun con_fwd_prop_elim ::"string \<Rightarrow> 'u rexp \<Rightarrow> 'u rexp list \<Rightarrow> bool" where
+fun con_fwd_prop_elim ::"string \<Rightarrow> 'u BA rexp \<Rightarrow> 'u BA rexp list \<Rightarrow> bool" where
 "con_fwd_prop_elim f r es = (if f = ''concat'' then lang (r) = List.foldl (*) (lang (hd es)) (map lang (tl es)) \<and> is_singleton (lang r) else False)"
 
-fun con_bwd_prop ::"string \<Rightarrow> 'u rexp \<Rightarrow> ('u rexp * 'u rexp) set" where
+fun con_bwd_prop ::"string \<Rightarrow> 'u BA rexp \<Rightarrow> ('u BA rexp * 'u BA rexp) set" where
 "con_bwd_prop f r = (if f = ''concat'' then pre_image_conc r else {})"
 
 value "\<Union>{{1}, {2::nat},{4}}"
 
 abbreviation msins ("_, _" [56,56] 56) where "x,M == insert x M"
 
-inductive One_SC :: \<open>'u form set set \<Rightarrow> bool\<close> (\<open>\<turnstile> _\<close> 0) where
+inductive One_SC :: \<open>'u BA form set set \<Rightarrow> bool\<close> (\<open>\<turnstile> _\<close> 0) where
   AlphaCon:      \<open>\<turnstile> {A,B,\<Gamma>} \<Longrightarrow> \<turnstile> {Con A B,\<Gamma>}\<close>
 | AlphaNegOr:    \<open>\<turnstile> {Neg A, Neg B, \<Gamma>} \<Longrightarrow> \<turnstile> {Neg (Dis A B), \<Gamma>}\<close>
 | AlphaOr:       \<open>\<turnstile> {A , \<Gamma>} \<Longrightarrow> \<turnstile> {B , \<Gamma>} \<Longrightarrow> \<turnstile> {Dis A B , \<Gamma>}\<close>
@@ -107,7 +107,7 @@ inductive One_SC :: \<open>'u form set set \<Rightarrow> bool\<close> (\<open>\<
 
 subsection \<open>Soundness\<close>
 
-lemma SC_soundness: \<open>\<turnstile> \<Gamma>S \<Longrightarrow>\<exists>\<Gamma>\<in> \<Gamma>S. \<forall>p \<in> \<Gamma>. eval e f p\<close>
+lemma SC_soundness: \<open>\<turnstile> \<Gamma>S \<Longrightarrow> \<exists>\<Gamma>\<in> \<Gamma>S. \<forall>p \<in> \<Gamma>. eval e f p\<close>
 proof (induct \<Gamma>S rule: One_SC.induct)
   case (AlphaCon A B \<Gamma>)
   then show ?case by auto
@@ -170,5 +170,9 @@ qed
 
 subsection \<open>Completeness\<close>
 
+theorem SC_completeness:
+  assumes \<open>\<exists>\<Gamma>\<in> \<Gamma>S. \<forall>p \<in> \<Gamma>. eval e f p\<close>
+  shows \<open>\<turnstile> \<Gamma>S\<close>
+  sorry
 
 end
